renamed inv23

src/proofs/no_slashable_attestations/supporting_lemmas/inv.dfy
@@ -1721,7 +1721,7 @@ module Att_Inv_With_Empty_Initial_Attestation_Slashing_DB
             && inv22_body(dvc)
     }
     
-    predicate inv23_body(dvc: DVCState)
+    predicate inv_slot_of_active_consensus_instance_is_lower_than_slot_of_latest_served_att_duty_body(dvc: DVCState)
     {
         dvc.latest_attestation_duty.isPresent()
         ==> ( forall k: Slot | k in dvc.attestation_consensus_engine_state.active_attestation_consensus_instances.Keys 
@@ -1730,11 +1730,11 @@ module Att_Inv_With_Empty_Initial_Attestation_Slashing_DB
             )
     }
 
-    predicate inv23(dv: DVState)
+    predicate inv_slot_of_active_consensus_instance_is_lower_than_slot_of_latest_served_att_duty(dv: DVState)
     {
         forall hn: BLSPubkey | hn in dv.honest_nodes_states.Keys ::
             && var dvc := dv.honest_nodes_states[hn];
-            && inv23_body(dvc)
+            && inv_slot_of_active_consensus_instance_is_lower_than_slot_of_latest_served_att_duty_body(dvc)
     }
 
     predicate concl_slot_of_active_consensus_instance_is_lower_than_slot_of_queued_att_duty_body(dvc: DVCState)
