src/proofs/no_slashable_attestations/supporting_lemmas/dv_next_invs_19_26.dfy
@@ -180,7 +180,7 @@ module DV_Next_Invs_19_26
         }   
     } 
 
-    lemma lemma_inv23_dv_next(
+    lemma lemma_inv_slot_of_active_consensus_instance_is_lower_than_slot_of_latest_served_att_duty_dv_next(
         dv: DVState,
         event: DV.Event,
         dv': DVState
@@ -194,8 +194,8 @@ module DV_Next_Invs_19_26
     requires inv17(dv)
     requires inv18(dv)
     requires inv22(dv)
-    requires inv23(dv)  
-    ensures inv23(dv')
+    requires inv_slot_of_active_consensus_instance_is_lower_than_slot_of_latest_served_att_duty(dv)  
+    ensures inv_slot_of_active_consensus_instance_is_lower_than_slot_of_latest_served_att_duty(dv')
     {        
         match event 
         {
@@ -212,20 +212,20 @@ module DV_Next_Invs_19_26
                         assert inv17_body(dvc);
                         assert inv18_body(dvc);
                         assert inv22_body(dvc);
-                        assert inv23_body(dvc);                                           
-                        lemma_inv23_f_serve_attestation_duty(dvc, attestation_duty, dvc');
-                        assert inv23_body(dvc');
+                        assert inv_slot_of_active_consensus_instance_is_lower_than_slot_of_latest_served_att_duty_body(dvc);                                           
+                        lemma_inv_slot_of_active_consensus_instance_is_lower_than_slot_of_latest_served_att_duty_f_serve_attestation_duty(dvc, attestation_duty, dvc');
+                        assert inv_slot_of_active_consensus_instance_is_lower_than_slot_of_latest_served_att_duty_body(dvc');
                         
                     case AttConsensusDecided(id, decided_attestation_data) => 
                         assert inv17_body(dvc);
                         assert inv18_body(dvc);
                         assert inv22_body(dvc);
-                        lemma_inv23_f_att_consensus_decided(dvc, id, decided_attestation_data, dvc');
-                        assert inv23_body(dvc');
+                        lemma_inv_slot_of_active_consensus_instance_is_lower_than_slot_of_latest_served_att_duty_f_att_consensus_decided(dvc, id, decided_attestation_data, dvc');
+                        assert inv_slot_of_active_consensus_instance_is_lower_than_slot_of_latest_served_att_duty_body(dvc');
                         
                     case ReceivedAttestationShare(attestation_share) =>                         
-                        lemma_inv23_f_listen_for_attestation_shares(dvc, attestation_share, dvc');
-                        assert inv23_body(dvc');
+                        lemma_inv_slot_of_active_consensus_instance_is_lower_than_slot_of_latest_served_att_duty_f_listen_for_attestation_shares(dvc, attestation_share, dvc');
+                        assert inv_slot_of_active_consensus_instance_is_lower_than_slot_of_latest_served_att_duty_body(dvc');
                        
                     case ImportedNewBlock(block) => 
                         assert inv17_body(dvc);
@@ -239,10 +239,10 @@ module DV_Next_Invs_19_26
                         assert inv18_body(dvc_mod);
                         lemma_inv22_add_block_to_bn(dvc, block, dvc_mod);
                         assert inv22_body(dvc_mod);
-                        lemma_inv23_add_block_to_bn(dvc, block, dvc_mod);
-                        assert inv23_body(dvc_mod);
-                        lemma_inv23_f_listen_for_new_imported_blocks(dvc_mod, block, dvc');                        
-                        assert inv23_body(dvc');
+                        lemma_inv_slot_of_active_consensus_instance_is_lower_than_slot_of_latest_served_att_duty_add_block_to_bn(dvc, block, dvc_mod);
+                        assert inv_slot_of_active_consensus_instance_is_lower_than_slot_of_latest_served_att_duty_body(dvc_mod);
+                        lemma_inv_slot_of_active_consensus_instance_is_lower_than_slot_of_latest_served_att_duty_f_listen_for_new_imported_blocks(dvc_mod, block, dvc');                        
+                        assert inv_slot_of_active_consensus_instance_is_lower_than_slot_of_latest_served_att_duty_body(dvc');
 
                     case ResendAttestationShares =>                                                                      
 
