src/proofs/no_slashable_attestations/supporting_lemmas/proofs_intermediate_steps.dfy
@@ -164,7 +164,7 @@ module Proofs_Intermediate_Steps
     )    
     requires inv18(dv)
     requires inv22(dv)
-    requires inv23(dv)
+    requires inv_slot_of_active_consensus_instance_is_lower_than_slot_of_latest_served_att_duty(dv)
     ensures concl_slot_of_active_consensus_instance_is_lower_than_slot_of_queued_att_duty(dv)    
     {   
         forall hn: BLSPubkey | hn in dv.honest_nodes_states.Keys
